src/tls/TLSConstants.fst
@@ -498,7 +498,7 @@ let parseCipherSuiteAux b =
   | ( 0xc0z, 0x2fz ) -> Correct(CipherSuite Kex_ECDHE (Some RSASIG) (AEAD AES_128_GCM SHA256))
   | ( 0xc0z, 0x30z ) -> Correct(CipherSuite Kex_ECDHE (Some RSASIG) (AEAD AES_256_GCM SHA384))
   (**************************************************************************)
-  | ( 0xd0z, 0x01z ) -> Correct(CipherSuite Kex_PSK_ECDHE None (AEAD AES_128_GCM SHA256)
+  | ( 0xd0z, 0x01z ) -> Correct(CipherSuite Kex_PSK_ECDHE None (AEAD AES_128_GCM SHA256))
   | ( 0xd0z, 0x02z ) -> Correct(CipherSuite Kex_PSK_ECDHE None (AEAD AES_256_GCM SHA384))
 
   (**************************************************************************)
